maybe use a singleton structure wrapper for Vec?

backends/lean/Aeneas/Std/Vec.lean
@@ -21,43 +21,54 @@ namespace alloc.vec
 @[rust_type "alloc::vec::Vec"]
 -- def Vec (α : Type u) := { l : List α // l.length ≤ Usize.max }
 structure Vec (α : Type u) where
-  leng : Nat
-  list : ListN α leng
-  bound : leng ≤ Usize.max
+  slice : Slice α
 deriving BEq, ReflBEq, LawfulBEq, DecidableEq
 
-def Vec.val {α} (s : Vec α) : List α := s.list.toList
+@[simp]
+instance (α : Type u) : CoeOut (Vec α) (Slice α) where
+  coe := λ v => v.slice
 
-@[simp, grind ., grind! .]
-theorem Vec.property {α} (s : Vec α) : s.val.length ≤ Usize.max := by
-  simp [Vec.val, ListN_length]
-  apply s.bound
+-- @[simp]
+-- instance (α : Type u) : CoeOut (Slice α) (Vec α) where
+--   coe := λ s => {slice := s}
 
-def Vec.from {α} (l : List α) (h : l.length ≤ Usize.max) : Vec α :=
-  {
-    leng := l.length
-    list := .fromList l
-    bound := by assumption
-  }
+@[simp]
+instance (α : Type u) : CoeTail (Slice α) (Vec α) where
+  coe := λ s => {slice := s}
 
-@[simp, grind! ., grind .]
-theorem Vec.from_val {α} (l : List α) (h : l.length ≤ Usize.max)
-  : (Vec.from l h).val = l := by
-  simp [Vec.from, Vec.val, ListN.from_to_inverse]
+-- @[simp]
+-- instance (α : Type u) : Coe (Slice α) (Vec α) where
+--   coe := λ s => {slice := s}
 
-@[simp, grind! ., grind .]
-theorem Vec.val_from {α} (s : Vec α) h
-  : Vec.from s.val h = s := by
-  cases s
-  simp [val, Vec.from] at *
-  simp [ListN_length]
-  apply ListN.to_from_inverse
+example a (s : Slice a) : Vec a := s
+example a (s : Vec a) : Slice a := s
+example (α : Type u) : Vec α := (Slice.from [] (by simp))
+example a (s : Nat → Slice a) : Vec a := s 10
+example a (s : List a → Slice a) : Vec a := s []
+example a (s : ∀ {a}, List a → Slice a) : Vec a := @s a []
+example a (s : ∀ {a}, List a → Slice a) : Vec a := @s _ []
+example a (s : Slice a × Slice a) : Vec a × Vec a := s
+#check Slice.from
 
 /-- We need this to coerce vectors to lists without marking `Vec` as reducible.
     Also not that we *do not* want to mark `Vec` as reducible: it triggers issues.
 -/
-instance (α : Type u) : CoeOut (Vec α) (List α) where
-  coe := λ v => v.val
+-- TODO: do i need this?
+-- instance (α : Type u) : CoeOut (Vec α) (List α) where
+  -- coe := λ v => v.val
+
+-- TODO: clean
+-- instance [BEq α] : BEq (Vec α) := SubtypeBEq _
+
+-- instance [BEq α] [LawfulBEq α] : LawfulBEq (Vec α) := SubtypeLawfulBEq _
+
+def Vec.val {α} (v : Vec α) : List α := (Slice.val v)
+
+@[simp, grind ., grind! .]
+theorem Vec.property {α} (s : Vec α) : s.val.length ≤ Usize.max := by
+  -- simp [Slice.val, ListN_length]
+  -- apply s.bound
+  sorry
 
 theorem Vec.len_ineq {α : Type u} (v : Vec α) : v.val.length ≤ Usize.max := by
   cases v; simp[*]
@@ -72,7 +83,7 @@ example {a: Type u} (v : Vec a) : v.length ≤ Usize.max := by
   simp
 
 @[rust_fun "alloc::vec::{alloc::vec::Vec<@T>}::new" -canFail -lift]
-abbrev Vec.new (α : Type u): Vec α := .from [] (by simp)
+abbrev Vec.new (α : Type u): Vec α := (@Slice.from α [] (by simp))
 
 instance (α : Type u) : Inhabited (Vec α) := by
   constructor
@@ -130,10 +141,10 @@ abbrev Vec.get? {α : Type u} (v : Vec α) (i : Nat) : Option α := getElem? v i
 abbrev Vec.get! {α : Type u} [Inhabited α] (v : Vec α) (i : Nat) : α := getElem! v i
 
 def Vec.set {α : Type u} (v: Vec α) (i: Usize) (x: α) : Vec α :=
-  .from (v.val.set i.val x) (by have := v.property; simp [*])
+  ⟨ v.val.set i.val x, by have := v.property; simp [*] ⟩
 
 def Vec.set_opt {α : Type u} (v: Vec α) (i: Usize) (x: Option α) : Vec α :=
-  .from (v.val.set_opt i.val x) (by have := v.property; simp [*])
+  ⟨ v.val.set_opt i.val x, by have := v.property; simp [*] ⟩
 
 @[simp, scalar_tac_simps, simp_lists_hyps_simps, grind =, agrind =]
 theorem Vec.set_val_eq {α : Type u} (v: Vec α) (i: Usize) (x: α) :
@@ -150,7 +161,7 @@ def Vec.push {α : Type u} (v : Vec α) (x : α) : Result (Vec α)
   :=
   let nlen := List.length v.val + 1
   if h : nlen ≤ U32.max || nlen ≤ Usize.max then
-    ok (.from (List.concat v.val x) (by simp; scalar_tac))
+    ok ⟨ List.concat v.val x, by simp; scalar_tac ⟩
   else
     fail maximumSizeExceeded
 
@@ -163,7 +174,7 @@ theorem Vec.push_spec {α : Type u} (v : Vec α) (x : α) (h : v.val.length < Us
 @[rust_fun "alloc::vec::{alloc::vec::Vec<@T>}::insert" (keepParams := [true, false])]
 def Vec.insert {α : Type u} (v: Vec α) (i: Usize) (x: α) : Result (Vec α) :=
   if i.val < v.length then
-    ok (.from (v.val.set i x) (by have := v.property; simp [*]))
+    ok ⟨ v.val.set i x, by have := v.property; simp [*] ⟩
   else
     fail arrayOutOfBounds
 
@@ -186,24 +197,11 @@ theorem Vec.index_usize_spec {α : Type u} (v: Vec α) (i: Usize)
   simp at *
   simp [*]
 
-theorem Vec.eq_iff {α} (s0 s1 : Vec α) : s0 = s1 ↔ s0.val = s1.val := by
-  constructor
-  · grind
-  · intros p
-    simp [val] at p
-    have : s1.list ≍ s0.list := by
-      have := ListN.to_from_inverse (l:=s0.list)
-      have := ListN.to_from_inverse (l:=s1.list)
-      grind
-    cases s0; cases s1
-    simp at *
-    constructor <;> try grind [ListN_length]
-
 def Vec.update {α : Type u} (v: Vec α) (i: Usize) (x: α) : Result (Vec α) :=
   match v.val[i.val]? with
   | none => fail .arrayOutOfBounds
   | some _ =>
-    ok (.from (v.val.set i x) (by have := v.property; simp [*]))
+    ok ⟨ v.val.set i x, by have := v.property; simp [*] ⟩
 
 @[step]
 theorem Vec.update_spec {α : Type u} (v: Vec α) (i: Usize) (x : α)
@@ -235,13 +233,19 @@ theorem Vec.index_mut_usize_spec {α : Type u} (v: Vec α) (i: Usize)
 
 @[rust_fun "alloc::vec::{core::ops::index::Index<alloc::vec::Vec<@T>, @I, @O>}::index"
   (keepParams := [true,true,false, true])]
-def Vec.index {T I Output : Type} (inst : core.slice.index.SliceIndex I (Vec T) Output)
+def Vec.index {T I Output : Type} (inst : core.slice.index.SliceIndex I (Slice T) Output)
   (self : Vec T) (i : I) : Result Output :=
   inst.index i self
 
+-- TODO: clean this, this is to test if it can fix the following definition
+@[simp]
+instance (a b : Type u) [CoeOut a b] : CoeOut (Result a) (Result b) where
+  coe := sorry
+
+-- NOTE: this here is why the coerciion idea doesn't really work, i think
 @[rust_fun "alloc::vec::{core::ops::index::IndexMut<alloc::vec::Vec<@T>, @I, @O>}::index_mut"
   (keepParams := [true,true,false, true])]
-def Vec.index_mut {T I Output : Type} (inst : core.slice.index.SliceIndex I (Vec T) Output)
+def Vec.index_mut {T I Output : Type} (inst : core.slice.index.SliceIndex I (Slice T) Output)
   (self : Vec T) (i : I) :
   Result (Output × (Output → Vec T)) :=
   inst.index_mut i self
@@ -249,7 +253,7 @@ def Vec.index_mut {T I Output : Type} (inst : core.slice.index.SliceIndex I (Vec
 @[reducible,
   rust_trait_impl "core::ops::index::Index<alloc::vec::Vec<@T>, @T, @O>" (keepParams := [true, true, false, true])]
 def Vec.Index {T I Output : Type}
-  (inst : core.slice.index.SliceIndex I (Vec T) Output) :
+  (inst : core.slice.index.SliceIndex I (Slice T) Output) :
   core.ops.index.Index (alloc.vec.Vec T) I Output := {
   index := Vec.index inst
 }
@@ -257,115 +261,24 @@ def Vec.Index {T I Output : Type}
 @[reducible,
   rust_trait_impl "core::ops::index::IndexMut<alloc::vec::Vec<@T>, @T, @O>" (keepParams := [true, true, false, true])]
 def Vec.IndexMut {T I Output : Type}
-  (inst : core.slice.index.SliceIndex I (Vec T) Output) :
+  (inst : core.slice.index.SliceIndex I (Slice T) Output) :
   core.ops.index.IndexMut (alloc.vec.Vec T) I Output := {
   indexInst := Vec.Index inst
   index_mut := Vec.index_mut inst
 }
 
--- TODO: should i have this? is it only used in one place?
-/-- Small helper (this function doesn't model a specific Rust function) -/
-def Vec.clone {T : Type} (clone : T → Result T) (s : Slice T) : Result (Vec T) := do
-  let s' ← List.clone clone s.val
-  ok (.from s' (by simp))
-
-@[reducible, rust_trait_impl "core::slice::index::SliceIndex<usize, [@T], @T>"]
-def core.slice.index.SliceIndexUsizeVec (T : Type) :
-  core.slice.index.SliceIndex Usize (Vec T) T := {
-  sealedInst := core.slice.index.private_slice_index.SealedUsize
-  get := fun i s => ok s[i]?
-  get_mut := fun i s => ok (s[i]?, s.set_opt i)
-  get_unchecked := fun _ _ => fail .undef
-  get_unchecked_mut := fun _ _ => fail .undef
-  index := fun i s => Vec.index_usize s i
-  index_mut := fun i s => Vec.index_mut_usize s i
-}
-
-@[reducible, rust_trait_impl "core::slice::index::private_slice_index::Sealed<core::ops::range::RangeTo<usize>>"]
-def core.slice.index.private_slice_index.SealedRangeToUsize :
-  core.slice.index.private_slice_index.Sealed (core.ops.range.RangeTo Usize)
-  := {}
-
-@[rust_fun "core::slice::index::{core::slice::index::SliceIndex<core::ops::range::RangeTo<usize>, [@T], [@T]>}::get"]
-def core.slice.index.SliceIndexRangeToUsizeVec.get
-  {T : Type} (r : core.ops.range.RangeTo Usize) (s : Vec T) : Result (Option (Vec T)) :=
-  if r.end ≤ s.length then
-    ok (some (.from (s.val.slice 0 r.end) (by scalar_tac)))
-  else ok none
-
-@[rust_fun "core::slice::index::{core::slice::index::SliceIndex<core::ops::range::RangeTo<usize>, [@T], [@T]>}::get_mut"]
-def core.slice.index.SliceIndexRangeToUsizeVec.get_mut
-  {T : Type} (r : core.ops.range.RangeTo Usize) (s : Vec T) :
-  Result ((Option (Vec T)) × (Option (Vec T) → Vec T)) :=
-  if r.end ≤ s.length then
-    ok (some (.from (s.val.slice 0 r.end) (by scalar_tac)),
-        fun s' =>
-        match s' with
-        | none => s
-        | some s' =>
-          if h: s'.length = r.end then
-            .from (List.setSlice! s.val 0 s'.val) (by simp)
-          else s )
-  else ok (none, fun _ => s)
-
-@[rust_fun "core::slice::index::{core::slice::index::SliceIndex<core::ops::range::RangeTo<usize>, [@T], [@T]>}::get_unchecked"]
-def core.slice.index.SliceIndexRangeToUsizeVec.get_unchecked
-  {T : Type} (_ : core.ops.range.RangeTo Usize) (_ : ConstRawPtr (Vec T)) : Result (ConstRawPtr (Vec T)) :=
-  -- TODO: update once we make the model of computation more stateful (for now we just fail)
-  fail .undef
-
-@[rust_fun "core::slice::index::{core::slice::index::SliceIndex<core::ops::range::RangeTo<usize>, [@T], [@T]>}::get_unchecked_mut"]
-def core.slice.index.SliceIndexRangeToUsizeVec.get_unchecked_mut
-  {T : Type} (_ : core.ops.range.RangeTo Usize) (_ : MutRawPtr (Vec T)) :
-  Result (MutRawPtr (Vec T)) :=
-  -- TODO: update once we make the model of computation more stateful (for now we just fail)
-  fail .undef
-
-@[rust_fun "core::slice::index::{core::slice::index::SliceIndex<core::ops::range::RangeTo<usize>, [@T], [@T]>}::index"]
-def core.slice.index.SliceIndexRangeToUsizeVec.index
-  {T : Type} (r : core.ops.range.RangeTo Usize) (s : Vec T) : Result (Vec T) :=
-  if r.end ≤ s.length then
-    ok (.from (s.val.slice 0 r.end) (by scalar_tac))
-  else fail .panic
-
-@[rust_fun "core::slice::index::{core::slice::index::SliceIndex<core::ops::range::RangeTo<usize>, [@T], [@T]>}::index_mut"]
-def core.slice.index.SliceIndexRangeToUsizeVec.index_mut
-  {T : Type} (r : core.ops.range.RangeTo Usize) (s : Vec T) :
-  Result ((Vec T) × (Vec T → Vec T)) :=
-  if r.end ≤ s.length then
-    ok (.from (s.val.slice 0 r.end) (by scalar_tac),
-        /- The back function expects a slice of the same length as the returned subslice.
-           We don't enforce this with a guard because we want totality; `setSlice!` handles
-           any length gracefully. The model is correct when this condition holds, which is
-           always the case for code generated by Aeneas. -/
-        fun s' => .from (List.setSlice! s.val 0 s'.val) (by simp))
-  else fail .panic
-
-@[reducible, rust_trait_impl "core::slice::index::SliceIndex<core::ops::range::RangeTo<usize>, [@T], [@T]>"]
-def core.slice.index.SliceIndexRangeToUsizeVec (T : Type) :
-  core.slice.index.SliceIndex (core.ops.range.RangeTo Usize) (Vec T) (Vec
-  T) := {
-  sealedInst := core.slice.index.private_slice_index.SealedRangeToUsize
-  get := core.slice.index.SliceIndexRangeToUsizeVec.get
-  get_mut := core.slice.index.SliceIndexRangeToUsizeVec.get_mut
-  get_unchecked := core.slice.index.SliceIndexRangeToUsizeVec.get_unchecked
-  get_unchecked_mut := core.slice.index.SliceIndexRangeToUsizeVec.get_unchecked_mut
-  index := core.slice.index.SliceIndexRangeToUsizeVec.index
-  index_mut := core.slice.index.SliceIndexRangeToUsizeVec.index_mut
-}
-
 @[simp, step_simps]
 theorem Vec.index_slice_index {α : Type} (v : Vec α) (i : Usize) :
-  Vec.index (core.slice.index.SliceIndexUsizeVec α) v i =
+  Vec.index (core.slice.index.SliceIndexUsizeSlice α) v i =
   Vec.index_usize v i := by
-  simp [Vec.index, Vec.index_usize]
+  simp [Vec.index, Vec.index_usize, Slice.index_usize]
   rfl
 
 @[simp, step_simps]
 theorem Vec.index_mut_slice_index {α : Type} (v : Vec α) (i : Usize) :
-  Vec.index_mut (core.slice.index.SliceIndexUsizeVec α) v i =
+  Vec.index_mut (core.slice.index.SliceIndexUsizeSlice α) v i =
   index_mut_usize v i := by
-  simp [Vec.index_mut, Vec.index_mut_usize, Slice.index_mut_usize, Slice.index_mut_usize]
+  simp [Vec.index_mut, Vec.index_mut_usize, Slice.index_mut_usize]
   rfl
 
 -- Vec index/index_mut with RangeTo
@@ -373,7 +286,7 @@ theorem Vec.index_mut_slice_index {α : Type} (v : Vec α) (i : Usize) :
 @[step]
 theorem Vec.index_RangeTo_spec {α : Type} (v : Vec α) (r : core.ops.range.RangeTo Usize)
     (h : r.end ≤ v.length) :
-    Vec.index (core.slice.index.SliceIndexRangeToUsizeVec α) v r
+    Vec.index (core.slice.index.SliceIndexRangeToUsizeSlice α) v r
     ⦃ s1 =>
       s1.val = v.val.slice 0 r.end ∧
       s1.length = r.end ⦄ := by
@@ -382,23 +295,10 @@ theorem Vec.index_RangeTo_spec {α : Type} (v : Vec α) (r : core.ops.range.Rang
   exact this
 
 @[step]
-theorem core.slice.index.SliceIndexRangeToUsizeVec.index.step_spec
-    (r : core.ops.range.RangeTo Usize) (s : Vec α) (h : r.end ≤ s.length) :
-  core.slice.index.SliceIndexRangeToUsizeVec.index r s
-    ⦃ s1 =>
-      s1.val = s.val.slice 0 r.end ∧
-      s1.length = r.end ⦄ := by
-  simp only [index]
-  split
-  · simp only [spec_ok, Slice.length, true_and]
-    simp; scalar_tac
-  · scalar_tac
-
-@[step]
 theorem Vec.index_mut_RangeTo_spec {α : Type} (v : Vec α) (r : core.ops.range.RangeTo Usize)
     (h : r.end ≤ v.length) :
-    Vec.index_mut (core.slice.index.SliceIndexRangeToUsizeVec α) v r
-    ⦃ (s1 : Vec α) (back : Vec α → Vec α) =>
+    Vec.index_mut (core.slice.index.SliceIndexRangeToUsizeSlice α) v r
+    ⦃ (s1 : Slice α) (back : Slice α → Vec α) =>
       s1.val = v.val.slice 0 r.end ∧
       s1.length = r.«end» ∧
       ∀ s', (back s').val = v.val.setSlice! 0 s'.val ⦄ := by
@@ -441,7 +341,8 @@ theorem Vec.index_Range_spec {α : Type} (v : Vec α) (r : core.ops.range.Range 
       s1.val = v.val.slice r.start r.end ∧
       s1.length = r.end - r.start ⦄ := by
   simp only [Vec.index]
-  have := core.slice.index.SliceIndexRangeUsizeSlice.index.step_spec r v h0 h1
+  -- TODO here with the implicit as well
+  have := @core.slice.index.SliceIndexRangeUsizeSlice.index.step_spec α r v h0 h1
   exact this
 
 @[step]
@@ -451,7 +352,8 @@ theorem Vec.index_mut_Range_spec {α : Type} (v : Vec α) (r : core.ops.range.Ra
     ⦃ (s1 : Slice α) (back : Slice α → Vec α) =>
       s1.val = v.val.slice r.start r.end ∧
       s1.length = r.end - r.start ∧
-      ∀ s2, back s2 = Slice.setSlice! v r.start.val s2 ⦄ := by
+      -- TODO: here i had to put implicit α parameter, TODO: clean this up if i found a way to not do that
+      ∀ s2, back s2 = @Slice.setSlice! α v r.start.val s2 ⦄ := by
   simp only [Vec.index_mut]
   have := core.slice.index.SliceIndexRangeUsizeSlice.index_mut.step_spec r v h0 h1
   exact this
@@ -461,13 +363,14 @@ end alloc.vec
 @[rust_fun "alloc::slice::{[@T]}::to_vec"]
 def alloc.slice.Slice.to_vec
   {T : Type} (cloneInst : core.clone.Clone T) (s : Slice T) : Result (alloc.vec.Vec T) := do
-  alloc.vec.Vec.clone cloneInst.clone s
+  Slice.clone cloneInst.clone s
 
 @[step]
 theorem alloc.slice.Slice.to_vec_spec {T : Type} (cloneInst : core.clone.Clone T) (s : Slice T)
   (h : ∀ x ∈ s.val, cloneInst.clone x = ok x) :
   alloc.slice.Slice.to_vec cloneInst s ⦃ s' => s = s'⦄ := by
   simp only [to_vec]
+  simp
   exact (Slice.clone_spec h)
 
 @[rust_fun "alloc::slice::{[@T]}::into_vec" -canFail -lift (keepParams := [true, false])]
@@ -479,7 +382,7 @@ def alloc.vec.from_elem
   {T : Type} (cloneInst : core.clone.Clone T)
   (x : T) (n : Usize) : Result (alloc.vec.Vec T) := do
   let l ← List.clone cloneInst.clone (List.replicate n.val x)
-  ok (.from l.val (by have := l.property; scalar_tac))
+  ok ⟨ l.val, by have := l.property; scalar_tac ⟩
 
 @[step]
 theorem alloc.vec.from_elem_spec {T : Type} (cloneInst : core.clone.Clone T)
@@ -500,7 +403,7 @@ def alloc.vec.Vec.extend_from_slice {T : Type} (cloneInst : core.clone.Clone T)
   if h : v.length + s.length ≤ Usize.max then do
     match h' : Slice.clone cloneInst.clone s with
     | ok s' =>
-      ok (.from (v.val ++ s'.val) (by have := Slice.clone_length h'; scalar_tac))
+      ok ⟨ v.val ++ s'.val , by have := Slice.clone_length h'; scalar_tac ⟩
     | fail e => fail e
     | div => div
   else fail .panic
@@ -508,7 +411,7 @@ def alloc.vec.Vec.extend_from_slice {T : Type} (cloneInst : core.clone.Clone T)
 @[rust_fun "alloc::vec::{core::ops::deref::Deref<alloc::vec::Vec<@T>, [@T]>}::deref"
            -canFail -lift (keepParams := [true, false])]
 def alloc.vec.Vec.deref {T : Type} (v : alloc.vec.Vec T) : Slice T :=
-  .from v.val v.property
+  ⟨ v.val, v.property ⟩
 
 @[reducible, rust_trait_impl "core::ops::deref::Deref<alloc::vec::Vec<@T>, [@T]>" (keepParams := [true, false])]
 def core.ops.deref.DerefVec {T : Type} : core.ops.deref.Deref (alloc.vec.Vec T) (Slice T) := {
@@ -519,7 +422,7 @@ def core.ops.deref.DerefVec {T : Type} : core.ops.deref.Deref (alloc.vec.Vec T) 
            -canFail (keepParams := [true, false])]
 def alloc.vec.Vec.deref_mut {T : Type} (v :  alloc.vec.Vec T) :
    (Slice T) × (Slice T → alloc.vec.Vec T) :=
-   (.from v.val v.property, λ s => .from s.val s.property)
+   (⟨ v.val, v.property ⟩, λ s => ⟨ s.val, s.property ⟩)
 
 @[reducible, rust_trait_impl "core::ops::deref::DerefMut<alloc::vec::Vec<@T>, [@T]>" (keepParams := [true, false])]
 def core.ops.deref.DerefMutVec {T : Type} :
@@ -532,10 +435,10 @@ def core.ops.deref.DerefMutVec {T : Type} :
 def alloc.vec.Vec.resize {T : Type} (cloneInst : core.clone.Clone T)
   (v : alloc.vec.Vec T) (new_len : Usize) (value : T) : Result (alloc.vec.Vec T) := do
   if new_len.val < v.length then
-    ok (.from (v.val.resize new_len value) (by scalar_tac))
+    ok ⟨ v.val.resize new_len value, by scalar_tac ⟩
   else
     let value ← cloneInst.clone value
-    ok (.from (v.val.resize new_len value) (by scalar_tac))
+    ok ⟨ v.val.resize new_len value, by scalar_tac ⟩
 
 @[step]
 theorem alloc.vec.Vec.resize_spec {T} (cloneInst : core.clone.Clone T)
@@ -552,7 +455,7 @@ theorem alloc.vec.Vec.resize_spec {T} (cloneInst : core.clone.Clone T)
 theorem alloc.vec.Vec.set_getElem!_eq α [Inhabited α] (x : alloc.vec.Vec α) (i : Usize) :
   x.set i x[i]! = x := by
   simp only [getElem!_Usize_eq]
-  simp only [set_val_eq, Vec.eq_iff, List.set_getElem!]
+  simp only [Vec, set_val_eq, Subtype.ext_iff, List.set_getElem!]
 
 @[simp↓, scalar_tac_simps, simp_lists_safe, grind =, agrind =]
 theorem alloc.vec.Vec.set_getElem_eq α (x : alloc.vec.Vec α) (i : Usize) (h : i.val < x.length) :
@@ -561,7 +464,7 @@ theorem alloc.vec.Vec.set_getElem_eq α (x : alloc.vec.Vec α) (i : Usize) (h : 
     simpa using h
   have hself : x.val.set i.val x.val[i.val] = x.val :=
     List.set_getElem_self (as := x.val) (i := i.val) (h := h')
-  simp only [Vec.eq_iff, set_val_eq] at hself ⊢
+  simp only [alloc.vec.Vec, Subtype.ext_iff, set_val_eq] at hself ⊢
   exact hself
 
 @[simp_lists_safe↓]
@@ -591,7 +494,7 @@ theorem alloc.vec.Vec.getElem_set_neq α (v : alloc.vec.Vec α) (i j : Usize) (x
   "alloc::vec::{core::convert::From<alloc::vec::Vec<@T>, [@T; @N]>}::from"]
 def alloc.vec.FromVecArray.from
   {T : Type} {N : Std.Usize} (a: Array T N) : Result (alloc.vec.Vec T) :=
-  ok (.from a.val (by scalar_tac))
+  ok ⟨ a.val, by scalar_tac ⟩
 
 @[reducible, rust_trait_impl
   "core::convert::From<alloc::vec::Vec<@T>, [@T; @N]>"]
@@ -602,7 +505,7 @@ def core.convert.FromVecArray (T : Type) (N : Std.Usize) : core.convert.From
 
 /- Source: '/rustc/library/alloc/src/vec/mod.rs', lines 3967:4-3967:33 -/
 @[rust_fun "alloc::vec::{core::convert::From<Box<[@T]>, alloc::vec::Vec<@T>>}::from" (keepParams := [true,false])]
-def alloc.vec.FromBoxSliceVec.from {T : Type} (v : alloc.vec.Vec T) : Result (Slice T) := ok (.from v.val v.property)
+def alloc.vec.FromBoxSliceVec.from {T : Type} (v : alloc.vec.Vec T) : Result (Slice T) := ok v
 
 @[step]
 theorem alloc.vec.FromBoxSliceVec.from_spec {T : Type} (v : alloc.vec.Vec T) :
@@ -616,18 +519,18 @@ def core.convert.FromBoxSliceVec (T : Type) :
 }
 
 def alloc.vec.Vec.setSlice! {α : Type u} (s : alloc.vec.Vec α) (i : ℕ) (s' : List α) : alloc.vec.Vec α :=
-  .from (s.val.setSlice! i s') (by simp)
+  ⟨s.val.setSlice! i s', by scalar_tac⟩
 
 @[simp, scalar_tac_simps, simp_scalar_safe, simp_lists_safe, grind =, agrind =]
 theorem alloc.vec.Vec.setSlice!_length {α : Type u} (s : alloc.vec.Vec α) (i : ℕ) (s' : List α) :
   (s.setSlice! i s').length = s.length := by
-  simp [Vec.length, Vec.setSlice!, List.length_setSlice!]
+  simp only [Vec.length, Vec.setSlice!, List.length_setSlice!]
 
 @[simp_lists_safe, grind =, agrind =]
 theorem alloc.vec.Vec.setSlice!_getElem!_prefix {α} [Inhabited α]
   (s : alloc.vec.Vec α) (s' : List α) (i j : ℕ) (h : j < i) :
   (s.setSlice! i s')[j]! = s[j]! := by
-  simp [Vec.setSlice!, Vec.getElem!_Nat_eq]
+  simp only [Vec.setSlice!, Vec.getElem!_Nat_eq]
   simp_lists
 
 @[simp_lists_safe, grind =, agrind =]
@@ -637,7 +540,7 @@ theorem alloc.vec.Vec.setSlice!_getElem_prefix {α}
   have hj' : j < (s.setSlice! i s').length := by
     simpa [Vec.setSlice!_length] using h.2
   have h1 : (s.setSlice! i s')[j]? = s[j]? := by
-    simp [Vec.getElem?_Nat_eq, Vec.setSlice!]
+    simp only [Vec.getElem?_Nat_eq, Vec.setSlice!]
     simp_lists [List.setSlice!_getElem?_prefix]
   simpa [Vec.getElem?_Nat_eq, Vec.getElem_Nat_eq,
     List.getElem?_eq_getElem hj', List.getElem?_eq_getElem h.2] using h1
@@ -646,7 +549,7 @@ theorem alloc.vec.Vec.setSlice!_getElem_prefix {α}
 theorem alloc.vec.Vec.setSlice!_getElem!_middle {α} [Inhabited α]
   (s : alloc.vec.Vec α) (s' : List α) (i j : ℕ) (h : i ≤ j ∧ j - i < s'.length ∧ j < s.length) :
   (s.setSlice! i s')[j]! = s'[j - i]! := by
-  simp [Vec.setSlice!, Vec.getElem!_Nat_eq]
+  simp only [Vec.setSlice!, Vec.getElem!_Nat_eq]
   simp_lists
 
 @[simp_lists_safe, grind =, agrind =]
@@ -657,7 +560,7 @@ theorem alloc.vec.Vec.setSlice!_getElem_middle {α}
     simpa [Vec.setSlice!_length] using h.2.2
   have hji : j - i < s'.length := h.2.1
   have h1 : (s.setSlice! i s')[j]? = s'[j - i]? := by
-    simp [Vec.getElem?_Nat_eq, Vec.setSlice!]
+    simp only [Vec.getElem?_Nat_eq, Vec.setSlice!]
     simp_lists [List.setSlice!_getElem?_middle]
   simpa [Vec.getElem?_Nat_eq, Vec.getElem_Nat_eq,
     List.getElem?_eq_getElem hj', List.getElem?_eq_getElem hji] using h1
@@ -665,7 +568,7 @@ theorem alloc.vec.Vec.setSlice!_getElem_middle {α}
 theorem alloc.vec.Vec.setSlice!_getElem!_suffix {α} [Inhabited α]
   (s : alloc.vec.Vec α) (s' : List α) (i j : ℕ) (h : i + s'.length ≤ j) :
   (s.setSlice! i s')[j]! = s[j]! := by
-  simp [Vec.setSlice!, Vec.getElem!_Nat_eq]
+  simp only [Vec.setSlice!, Vec.getElem!_Nat_eq]
   simp_lists
 
 theorem alloc.vec.Vec.setSlice!_getElem_suffix {α}
@@ -674,7 +577,7 @@ theorem alloc.vec.Vec.setSlice!_getElem_suffix {α}
   have hj' : j < (s.setSlice! i s').length := by
     simpa [Vec.setSlice!_length] using h.2
   have h1 : (s.setSlice! i s')[j]? = s[j]? := by
-    simp [Vec.getElem?_Nat_eq, Vec.setSlice!]
+    simp only [Vec.getElem?_Nat_eq, Vec.setSlice!]
     simp_lists [List.setSlice!_getElem?_suffix]
   simpa [Vec.getElem?_Nat_eq, Vec.getElem_Nat_eq,
     List.getElem?_eq_getElem hj', List.getElem?_eq_getElem h.2] using h1
@@ -770,7 +673,7 @@ namespace Tests
     (↑(↑divisor : ℕ) : ℤ) ≤
     (↑(↑slots : List (List α)).length : ℤ) * (↑(↑dividend : ℕ) : ℤ)
     := by
-    grind
+    scalar_tac
 
   example
     (v : alloc.vec.Vec U32)
